Preserve writability, mask specs and integration.

src/asn1/ASN1.Low.TLV.fst
@@ -2,20 +2,17 @@ module ASN1.Low.TLV
 
 open ASN1.Base
 open ASN1.Spec.Tag
-friend ASN1.Spec.Tag
 open ASN1.Spec.BOOLEAN
-friend ASN1.Spec.BOOLEAN
 open ASN1.Spec.NULL
 open ASN1.Spec.TLV
+open ASN1.Low.Base
+open ASN1.Low.Tag
+open ASN1.Low.BOOLEAN
 
-// open ASN1.Low.BOOLEAN
-// friend ASN1.Low.BOOLEAN
-
-include LowParse.Low.Base
-include LowParse.Low.Combinators
-include LowParse.Bytes
-include LowParse.Low.DER
-// include LowParse.Low.SeqBytes
+open LowParse.Low.Base
+open LowParse.Low.Combinators
+open LowParse.Bytes
+open LowParse.Low.DER
 
 module U8 = FStar.UInt8
 module U32 = FStar.UInt32
@@ -24,169 +21,54 @@ module HST = FStar.HyperStack.ST
 module MB = LowStar.Monotonic.Buffer
 module B = LowStar.Buffer
 module Cast = FStar.Int.Cast
-// open Lib.IntTypes
+
 open FStar.Integers
 
-#push-options "--z3rlimit 32"
-let size_t = U32.t
-let byte_t = U8.t
-
-/// NOTE: Adapted from `LowParse.Low.Bytes.store_bytes`
-/// TODO: Ensure writable
-inline_for_extraction
-let store_seqbytes
-  (src: bytes)
-  (src_from src_to: size_t)
-  (#rrel #rel: _)
-  (dst: B.mbuffer byte_t rrel rel)
-  (dst_pos: size_t)
-: HST.Stack unit
-  (requires (fun h ->
-    B.live h dst /\
-    U32.v src_from <= U32.v src_to /\ U32.v src_to <= Seq.length src /\
-    U32.v dst_pos + (U32.v src_to - U32.v src_from) <= B.length dst /\
-    writable dst (U32.v dst_pos) (U32.v dst_pos + (U32.v src_to - U32.v src_from)) h
-  ))
-  (ensures (fun h _ h' ->
-    B.modifies (B.loc_buffer_from_to dst dst_pos (dst_pos `U32.add` (src_to `U32.sub` src_from))) h h' /\
-    Seq.slice (B.as_seq h' dst) (U32.v dst_pos) (U32.v dst_pos + (U32.v src_to - U32.v src_from)) == Seq.slice (src) (U32.v src_from) (U32.v src_to)
-  ))
-= let h0 = HST.get () in
-  HST.push_frame ();
-  let h1 = HST.get () in
-  let bi = B.alloca 0ul 1ul in
-  let h2 = HST.get () in
-  let len = src_to `U32.sub` src_from in
-  C.Loops.do_while
-    (fun h stop ->
-      B.modifies (B.loc_union (B.loc_region_only true (HS.get_tip h1)) (B.loc_buffer_from_to dst dst_pos (dst_pos `U32.add` len))) h2 h /\
-      B.live h bi /\ (
-      let i = Seq.index (B.as_seq h bi) 0 in
-      U32.v i <= U32.v len /\
-      writable dst (U32.v dst_pos) (U32.v dst_pos + U32.v len) h /\
-      Seq.slice (B.as_seq h dst) (U32.v dst_pos) (U32.v dst_pos + U32.v i) `Seq.equal` Seq.slice (src) (U32.v src_from) (U32.v src_from + U32.v i) /\
-      (stop == true ==> i == len)
-    ))
-    (fun _ ->
-      let i = B.index bi 0ul in
-      if i = len
-      then true
-      else begin
-        let x = Seq.index src (v src_from + v i) in
-        mbuffer_upd dst (Ghost.hide (U32.v dst_pos)) (Ghost.hide (U32.v dst_pos + U32.v len)) (dst_pos `U32.add` i) x;
-        let i' = i `U32.add` 1ul in
-        B.upd bi 0ul i';
-        let h' = HST.get () in
-        Seq.lemma_split (Seq.slice (B.as_seq h' dst) (U32.v dst_pos) (U32.v dst_pos + U32.v i')) (U32.v i);
-        i' = len
-      end
-    )
-    ;
-  HST.pop_frame ()
-
-#pop-options
-
-#push-options "--z3rlimit 64"
-
-// [@unifier_hint_injective]
+// /// NOTE: Inlining all low-level serializers for now
 // inline_for_extraction
-// let serializer32_backwards
-//   (#k: parser_kind)
-//   (#t: Type)
-//   (#p: parser k t)
-//   (s: serializer p)
-// : Tot Type
-// = (x: t) ->
-//   (#rrel: _) -> (#rel: _) ->
-//   (b: B.mbuffer byte_t rrel rel) ->
-//   (pos: size_t) ->
-//   HST.Stack (offset: size_t)
-//   (* NOTE: b[pos - offset] is not written and b[pos - offset + 1] ~ b[pos] are written.
-//            Which means `offset` could at most be `pos + 1`?*)
-//   (requires fun h ->
-//     let offset = Seq.length (serialize s x) in
-//     B.live h b /\
-//     (* NOTE: 1) a valid `pos` should be in range [0, |b|),
-//              2) a valid `offset` should be in range [0, pos + 1],
-//              3) the slice gonna to be written is b[pos - offset + 1, pos]. *)
-//     0 <= v pos /\ v pos < B.length b /\
-//     0 <= offset /\ offset <= v pos + 1 /\
-//     writable
-//     (* buf *) b
-//     (* from*) (v pos - offset + 1)
-//     (* exto*) (v pos + 1)
-//     (* mem *) h)
-//   (ensures fun h offset h' ->
-//     let sx = serialize s x in
-//     Seq.length sx == v offset /\
-//     B.modifies (B.loc_buffer_from_to b (pos - offset + 1) (pos + 1)) h h' /\
-//     B.live h b /\
-//     Seq.slice (B.as_seq h' b) (v pos - v offset) (v pos) `Seq.equal` sx)
+// let serialize32_asn1_value_backwards'
+//   (x: valid_asn1_TL)
+// : serializer32_backwards (serialize_asn1_value x)
+// = fun (value: asn1_value_of_TL x)
+//     (#rrel #rel: _)
+//     (b: B.mbuffer byte_t rrel rel)
+//     (pos: size_t)
+// ->  let a, offset = x in
+//     (* Prf *) serialize_asn1_value_unfold x value;
+//     (* Prf *)
+//     (* Prf *) assert (v offset == Seq.length (serialize (serialize_asn1_value x) value));
+//     [@inline_let] let gstart = Ghost.hide (v (pos - offset)) in
+//     [@inline_let] let gend   = Ghost.hide (v pos) in
+//     let i = pos - offset in
+//     let h0 = HST.get () in
+//     let offset = match a with
+//     | BOOLEAN      -> ( serialize_asn1_boolean_unfold
+//                         mbuffer_upd
+//                         (* buf *) b
+//                         (*start*) gstart
+//                         (* end *) gend
+//                         (* pos *) i
+//                         (*  v  *) (encode_asn1_boolean (BOOLEAN_VALUE?.b value))
+//                       ; (* return *) offset )
 
-[@unifier_hint_injective]
-inline_for_extraction
-let serializer32_backwards
-  (#k: parser_kind)
-  (#t: Type)
-  (#p: parser k t)
-  (s: serializer p)
-: Tot Type
-= (x: t) ->
-  (#rrel: _) -> (#rel: _) ->
-  (b: B.mbuffer byte_t rrel rel) ->
-  (pos: size_t) ->
-  HST.Stack (offset: size_t)
-  (* NOTE: b[pos] is already written, and b[pos - offset, pos - 1] will be written. *)
-  (requires fun h ->
-    let offset = Seq.length (serialize s x) in
-    B.live h b /\
-    offset <= v pos /\ v pos <= B.length b /\
-    writable b (v pos - offset) (v pos) h)
-  (ensures fun h offset h' ->
-    let sx = serialize s x in
-    Seq.length sx == v offset /\
-    B.modifies (B.loc_buffer_from_to b (pos - offset) (pos)) h h' /\
-    // (forall (i:nat{0 <= i /\ i < B.length b /\ (i < v (pos - offset) \/ v pos <= i)}).
-    //   let s0 = B.as_seq h b in
-    //   let s1 = B.as_seq h' b in
-    //   s0.[i] == s1.[i]) /\
-    B.live h b /\
-    Seq.slice (B.as_seq h' b) (v pos - v offset) (v pos) `Seq.equal` sx)
+//     | NULL         -> ( (* return *) offset )
 
-/// NOTE: Inlining all low-level serializers for now
-inline_for_extraction
-let serialize32_asn1_value_backwards'
-  (x: valid_asn1_TL) (* FIXME: I doubt if we could know this ahead. *)
-: serializer32_backwards (serialize_asn1_value x)
-= fun (value: asn1_value_of_TL x)
-    (#rrel #rel: _)
-    (b: B.mbuffer byte_t rrel rel)
-    (pos: size_t)
-->  let a, offset = x in
-    (* Prf *) serialize_asn1_value_unfold x value;
-    (* Prf *) assert (v offset == Seq.length (serialize (serialize_asn1_value x) value));
-    [@inline_let] let gstart = Ghost.hide (v (pos - offset)) in
-    [@inline_let] let gend   = Ghost.hide (v pos) in
-    [@inline_let] let i      = pos - offset in
-    // (* Prf *) assert (Ghost.reveal gstart <= v i);
-    match a with
-    | BOOLEAN      -> ( mbuffer_upd
-                        (* buf *) b
-                        (*start*) gstart
-                        (* end *) gend
-                        (* pos *) i
-                        (*  v  *) (encode_asn1_boolean (BOOLEAN_VALUE?.b value))
-                      ; (* return *) offset )
+//     | OCTET_STRING -> admit(); ( store_seqbytes
+//                         (* src *) (OCTET_STRING_VALUE?.s value)
+//                         (* from*) 0ul
+//                         (* to  *) offset
+//                         (* dst *) b
+//                         (* pos *) i
+//                       ; (* return *) offset ) in
+//     let h1 = HST.get () in
+//     (* Prf *) writable_modifies
+//               (* buf *) b
+//               (* new *) (v (pos - offset)) (v (pos))
+//               (* mem *) h0
+//               (* loc *) B.loc_none
+//               (* mem'*) h1;
 
-    | NULL         -> ( (* return *) offset )
-
-    | OCTET_STRING -> ( store_seqbytes
-                        (* src *) (OCTET_STRING_VALUE?.s value)
-                        (* from*) 0ul
-                        (* to  *) offset
-                        (* dst *) b
-                        (* pos *) i
-                      ; (* return *) offset )
+// (*return*) offset
 
 let offset_of_asn1_value
   (value: asn1_value)
@@ -197,11 +79,7 @@ let offset_of_asn1_value
   | NULL_VALUE _           -> 0ul
   | OCTET_STRING_VALUE l s -> u l (* <-- FIXME!*)
 
-let offset_of_asn1_tag
-  (tag: asn1_type)
-: Tot (l: size_t{v l == Seq.length (serialize (serialize_asn1_tag ()) tag)})
-= 1ul (* <-- Maybe FIXME *)
-
+#push-options "--query_stats --z3rlimit 32"
 inline_for_extraction
 let serialize32_asn1_value_backwards
   (#value_: asn1_value)
@@ -218,17 +96,23 @@ let serialize32_asn1_value_backwards
     let i      = pos - offset in
     // (* Prf *) assert (Ghost.reveal gstart <= v i);
     match value with
-    | BOOLEAN_VALUE x        -> ( mbuffer_upd
+    | BOOLEAN_VALUE x        -> ( serialize32_asn1_boolean_backwards ()
+                                  (*  x  *) x
                                   (* buf *) b
-                                  (*start*) gstart
-                                  (* end *) gend
-                                  (* pos *) i
-                                  (*  v  *) (encode_asn1_boolean x)
-                                ; (* return *) offset )
+                                  (* pos *) pos )
+                                // ( serialize_asn1_boolean_unfold x;
+                                //   serialize_u8_spec (encode_asn1_boolean x);
+                                //   mbuffer_upd
+                                //   (* buf *) b
+                                //   (*start*) gstart
+                                //   (* end *) gend
+                                //   (* pos *) i
+                                //   (*  v  *) (encode_asn1_boolean x)
+                                // ; (* return *) offset )
 
     | NULL_VALUE n           -> ( (* return *) offset )
 
-    | OCTET_STRING_VALUE l s -> ( store_seqbytes
+    | OCTET_STRING_VALUE l s -> ( admit(); store_seqbytes
                                   (* src *) s
                                   (* from*) 0ul
                                   (* to  *) offset
@@ -308,12 +192,6 @@ let serialize_TL_backwards ()
               (* mem *) h0
               (* from*) (v (pos - offset_L))
               (* to  *) (v pos);
-    (* Prf *) writable_weaken
-              (* buf *) b
-              (*range*) (v (pos - offset_L - offset_T)) (v pos)
-              (* mem *) h0
-              (* from*) (v (pos - offset_L - offset_T))
-              (* to  *) (v (pos - offset_L));
     let _ = serialize32_bounded_der_length32_backwards
             (* min *) asn1_length_min
             (* max *) asn1_length_max
@@ -323,37 +201,25 @@ let serialize_TL_backwards ()
 
 /// serialize ASN.1 DER "Tag" `a` backwards into `b[pos - offset_L - offset_T, pos - offset_L - 1]`
     (* Prf *) let h1 = HST.get () in
-    (* Prf *) assert (B.modifies (B.loc_buffer_from_to b (pos - offset_L) (pos)) h0 h1);
-    (* NOTE: Need to prove the frame. *)
-    (* Prf *) B.modifies_buffer_from_to_elim
+    (* Prf *) writable_modifies
               (* buf *) b
-              (*frame*) (pos - offset_L - offset_T) (pos - offset_L)
-              (* new *) (B.loc_buffer_from_to
-                         (* buf *) b
-                         (*range*) (pos - offset_L) (pos))
-              (* mem *) h0 h1;
-    (* Prf *) assert (Seq.slice (B.as_seq h0 b) (v (pos - offset_L - offset_T)) (v (pos - offset_L))
-                      `Seq.equal`
-                      Seq.slice (B.as_seq h1 b) (v (pos - offset_L - offset_T)) (v (pos - offset_L)));
-    // (* Prf *) writable_ext b (v (pos - offset_L - offset_T)) (v (pos - offset_L)) h0 h1;
-    (* TODO: Should try `writable_replace_subseq`. *)
-    (* NOTE: `writable` for some reason is not preserved by `serialize32`, maybe that's the hard part. *)
-    (* Prf *) assume (writable b (v (pos - offset_L - offset_T)) (v (pos - offset_L)) h1); (* <-- FIXME *)
+              (* new *) (v (pos - offset_L - offset_T)) (v (pos))
+              (* mem *) h0
+              (* loc *) B.loc_none
+              (* mem'*) h1;
+    (* Prf *) writable_weaken
+              (* buf *) b
+              (*range*) (v (pos - offset_L - offset_T)) (v pos)
+              (* mem *) h1
+              (* from*) (v (pos - offset_L - offset_T))
+              (* to  *) (v (pos - offset_L));
+
     let _ = serialize32_asn1_tag_backwards ()
             (* tag *) a
             (* buf *) b
             (* pos *) (pos - offset_L) in
 
     (* Prf *) let h2 = HST.get () in
-    // (* Prf *) [@inline_let] let sx_L = serialize (serialize_bounded_der_length32 asn1_length_min asn1_length_max) len in
-    // (* Prf *) [@inline_let] let sx_T = serialize (serialize_asn1_tag ()) a in
-    // (* Prf *) [@inline_let] let sx_TL = serialize serialize_TL x in
-    (* Prf *) assert (B.modifies (B.loc_buffer_from_to b (pos - offset_L) (pos)) h0 h1);
-    (* Prf *) assert (B.modifies (B.loc_buffer_from_to b (pos - offset_L - offset_T) (pos - offset_L)) h1 h2);
-    (* Prf *) assert (Seq.slice (B.as_seq h1 b) (v (pos - offset_L)) (v pos)
-                      `Seq.equal`
-                      serialize (serialize_bounded_der_length32 asn1_length_min asn1_length_max) len);
-    (* NOTE: Need to prove the frame. *)
     (* Prf *) B.modifies_buffer_from_to_elim
               (* buf *) b
               (*frame*) (pos - offset_L) (pos)
@@ -361,23 +227,6 @@ let serialize_TL_backwards ()
                          (* buf *) b
                          (*range*) (pos - offset_L - offset_T) (pos - offset_L))
               (* mem *) h1 h2;
-    (* Prf *) assert (Seq.slice (B.as_seq h1 b) (v (pos - offset_L)) (v pos)
-                      `Seq.equal`
-                      Seq.slice (B.as_seq h2 b) (v (pos - offset_L)) (v pos));
-    (* Prf *) assert (Seq.slice (B.as_seq h2 b) (v (pos - offset_L)) (v pos)
-                      `Seq.equal`     (* ^^^ FIXME *)
-                      serialize (serialize_bounded_der_length32 asn1_length_min asn1_length_max) len);
-    (* Prf *) assert (Seq.slice (B.as_seq h2 b) (v (pos - offset_L - offset_T)) (v (pos - offset_L))
-                      `Seq.equal`
-                      serialize (serialize_asn1_tag ()) a);
-    (* Prf *) assert ((serialize (serialize_asn1_tag ()) a
-                       `Seq.append`
-                       serialize (serialize_bounded_der_length32 asn1_length_min asn1_length_max) len)
-                       `Seq.equal`
-                       serialize serialize_TL x);
-    (* Prf *) assert (Seq.slice (B.as_seq h2 b) (v (pos - offset_L - offset_T)) (v pos)
-                      `Seq.equal`
-                      serialize serialize_TL x);
 
 /// return offset
 (*return*) (offset_L + offset_T)
