src/asn1/ASN1.Spec.BOOLEAN.fsti
@@ -1,40 +1,55 @@
 module ASN1.Spec.BOOLEAN
 
-include LowParse.Spec.Base
-include LowParse.Spec.Combinators
-include LowParse.Spec.Int
+open LowParse.Spec.Base
+open LowParse.Spec.Combinators
+open LowParse.Spec.Int
 
-include ASN1.Base
+open ASN1.Base
 
 (* BOOLEAN primitive *)
-val encode_asn1_boolean
-  (b: bool)
-: Tot byte
+val filter_asn1_boolean
+  (b: byte)
+: Ghost bool
+  (requires True)
+  (ensures fun r -> r == (b = 0xFFuy || b = 0x00uy))
 
-val decode_asn1_boolean
-  (bs: bytes{Seq.length bs == 1})
-: Tot (option bool)
+let valid_asn1_boolean_byte = parse_filter_refine filter_asn1_boolean
 
-val decode_asn1_boolean_injective: unit -> Lemma (
-  make_constant_size_parser_precond 1 bool decode_asn1_boolean
-)
+val synth_asn1_boolean
+    (b: parse_filter_refine filter_asn1_boolean)
+: Ghost bool
+  (requires True)
+  (ensures fun x -> x == (b = 0xFFuy))
 
-(* NOTE: Expose kinds *)
-let parse_asn1_boolean_kind: parser_kind = constant_size_parser_kind 1
+val synth_asn1_boolean_inverse
+  (x: bool)
+: Ghost (b: parse_filter_refine filter_asn1_boolean{synth_asn1_boolean b == x})
+  (requires True)
+  (ensures fun b -> synth_asn1_boolean b == x)
+
+let parse_asn1_boolean_kind = strong_parser_kind 1 1 None
 val parse_asn1_boolean
 : parser parse_asn1_boolean_kind bool
 
 val parse_asn1_boolean_unfold
   (input: bytes)
 : Lemma (
+  parser_kind_prop parse_asn1_boolean_kind parse_asn1_boolean /\
   parse parse_asn1_boolean input ==
  (match parse parse_u8 input with
-  | Some (0xFFuy, 1) -> Some (true,  1)
-  | Some (0x00uy, 1) -> Some (false, 1)
-  | _                -> None)
-)
+  | Some (x, consumed) -> if filter_asn1_boolean x then
+                          ( Some (synth_asn1_boolean x, consumed) )
+                          else
+                          ( None )
+  | None -> None))
 
 val serialize_asn1_boolean
 : serializer parse_asn1_boolean
 
-// val synth_asn1_boolean_value: b: bool -> value: asn1_value{BOOLEAN_VALUE? value /\ BOOLEAN_VALUE}
+val serialize_asn1_boolean_unfold
+  (b: bool)
+: Lemma (
+  serialize serialize_asn1_boolean b
+  `Seq.equal`
+  serialize serialize_u8 (synth_asn1_boolean_inverse b))
+
