src/asn1/ASN1.Spec.Tag.fst
@@ -1,18 +1,41 @@
 module ASN1.Spec.Tag
 
-include LowParse.Spec.Base
-include LowParse.Spec.Combinators
-include LowParse.Spec.Int
-friend  LowParse.Spec.Int
+open LowParse.Spec.Base
+open LowParse.Spec.Combinators
+open LowParse.Spec.Int
 
-include ASN1.Base
+open ASN1.Base
 
 (* Tag parser primitive *)
 
-/// ASN.1 DER Tag Encoder
-let asn1_tag_of_type
+let filter_asn1_tag
+  (b: byte)
+: Ghost bool
+  (requires True)
+  (ensures fun r -> r == (b = 0x01uy || b = 0x04uy || b = 0x05uy))
+= match b with
+  | 0x01uy | 0x04uy | 0x05uy -> true
+  | _ -> false
+
+let synth_asn1_tag
+  (b: parse_filter_refine filter_asn1_tag)
+: Ghost asn1_type
+  (requires True)
+  (ensures fun a ->
+    a == (match b with
+          | 0x01uy -> BOOLEAN
+          | 0x04uy -> OCTET_STRING
+          | 0x05uy -> NULL))
+= match b with
+  | 0x01uy -> BOOLEAN
+  | 0x04uy -> OCTET_STRING
+  | 0x05uy -> NULL
+
+let synth_asn1_tag_inverse
   (a: asn1_type)
-: Tot byte
+: Ghost (b: parse_filter_refine filter_asn1_tag{a == synth_asn1_tag b})
+  (requires True)
+  (ensures fun b -> a == synth_asn1_tag b)
 = match a with
   | BOOLEAN      -> 0x01uy
   // | INTEGER      -> 0x02uy
@@ -22,107 +45,63 @@ let asn1_tag_of_type
   // | OID          -> 0x06uy
   // | SEQUENCE     -> 0x30uy
 
-let encode_asn1_tag
-= fun (a: asn1_type) -> asn1_tag_of_type a
-
-/// Generic ASN.1 DER Tag Parser
-///
-
-let decode_asn1_tag
-  (s: bytes {Seq.length s == 1})
-: Tot (option (asn1_type))
-= match s.[0] with
-  | 0x01uy -> Some BOOLEAN
-  // | 0x02uy -> Some INTEGER
-  // | 0x03uy -> Some BIT_STRING
-  | 0x04uy -> Some OCTET_STRING
-  | 0x05uy -> Some NULL
-  // | 0x06uy -> Some OID
-  // | 0x30uy -> Some SEQUENCE
-  | _      -> None
-
-let decode_asn1_tag_injective ()
-: Lemma (
-  forall (s1: bytes {Seq.length s1 == 1})
-    (s2: bytes {Seq.length s2 == 1}).
-  {:pattern (decode_asn1_tag s1); (decode_asn1_tag s2)}
-  let v1, v2 = decode_asn1_tag s1, decode_asn1_tag s2 in
-  (Some? v1 \/ Some? v2) /\ v1 == v2
-  ==> Seq.equal s1 s2)
-= ()
-
 let parse_asn1_tag
 : parser parse_asn1_tag_kind asn1_type
-= decode_asn1_tag_injective ();
-  make_constant_size_parser 1 asn1_type (decode_asn1_tag)
+= parse_u8
+  `parse_filter`
+  filter_asn1_tag
+  `parse_synth`
+  synth_asn1_tag
 
 let parse_asn1_tag_unfold
   (input: bytes)
 : Lemma (
   parse parse_asn1_tag input ==
  (match parse parse_u8 input with
-  | Some (x, 1) -> let d = decode_asn1_tag (Seq.create 1 x) in
-                   if Some? d then Some (Some?.v d, 1) else None
-  | _           -> None))
-= match parse parse_u8 input with
-  | Some (x, 1) -> ()
-  | _           -> ()
+  | Some (x, consumed) -> if filter_asn1_tag x then
+                          ( Some (synth_asn1_tag x, consumed) )
+                          else
+                          ( None )
+  | None -> None))
+= parser_kind_prop_equiv parse_asn1_tag_kind parse_asn1_tag;
+  parse_filter_eq
+  (* p  *) (parse_u8)
+  (* f  *) (filter_asn1_tag)
+  (* in *) (input);
+  parse_synth_eq
+  (* p1 *) (parse_u8
+            `parse_filter`
+            filter_asn1_tag)
+  (* f2 *) (synth_asn1_tag)
+  (* in *) (input)
 
-let serialize_asn1_tag ()
-: Tot (serializer parse_asn1_tag)
-= fun (a: asn1_type) -> Seq.create 1 (encode_asn1_tag a)
+let serialize_asn1_tag
+: serializer parse_asn1_tag
+= serialize_synth
+  (* p1 *) (parse_u8
+            `parse_filter`
+            filter_asn1_tag)
+  (* f2 *) (synth_asn1_tag)
+  (* s1 *) (serialize_u8
+            `serialize_filter`
+            filter_asn1_tag)
+  (* g1 *) (synth_asn1_tag_inverse)
+  (* prf*) ()
 
-/// Specialized ASN.1 DER Tag Parser
-///
-
-/// Specialized decoder
-let decode_the_asn1_tag
-  (a: asn1_type)
-  (s: bytes {Seq.length s == 1})
-: Tot (option (the_asn1_type a))
-= match a, s.[0] with
-  | BOOLEAN      , 0x01uy -> Some BOOLEAN
-  // | INTEGER      , 0x02uy -> Some INTEGER
-  // | BIT_STRING   , 0x03uy -> Some BIT_STRING
-  | OCTET_STRING , 0x04uy -> Some OCTET_STRING
-  | NULL         , 0x05uy -> Some NULL
-  // | OID          , 0x06uy -> Some OID
-  // | SEQUENCE     , 0x30uy -> Some SEQUENCE
-  | _                     -> None
-
-/// Decoder is injective
-let decode_the_asn1_tag_injective
+let serialize_asn1_tag_unfold
   (a: asn1_type)
 : Lemma (
-  forall (s1: bytes {Seq.length s1 == 1})
-    (s2: bytes {Seq.length s2 == 1}).
-  {:pattern (decode_the_asn1_tag a s1); (decode_the_asn1_tag a s2)}
-  let v1, v2 = decode_the_asn1_tag a s1, decode_the_asn1_tag a s2 in
-  (Some? v1 \/ Some? v2) /\ v1 == v2
-  ==> Seq.equal s1 s2)
-= ()
-
-/// Specialized parser
-let parse_the_asn1_tag
-  (a:asn1_type)
-: parser parse_asn1_tag_kind (the_asn1_type a)
-= decode_the_asn1_tag_injective a;
-  make_constant_size_parser 1 (the_asn1_type a) (decode_the_asn1_tag a)
-
-let parse_the_asn1_tag_unfold
-  (a: asn1_type)
-  (input: bytes)
-: Lemma (
-  parse (parse_the_asn1_tag a) input ==
- (match parse parse_u8 input with
-  | Some (x, 1) -> if x = asn1_tag_of_type a then Some (a, 1) else None
-  | _           -> None))
-= match parse parse_u8 input with
-  | Some (x, 1) -> ()
-  | _           -> ()
-
-/// Specialized serializer
-let serialize_the_asn1_tag
-  (a: asn1_type)
-: Tot (serializer (parse_the_asn1_tag a))
-= fun (a': the_asn1_type a) -> Seq.create 1 (encode_asn1_tag a')
+  serialize serialize_asn1_tag a
+  `Seq.equal`
+  serialize serialize_u8 (synth_asn1_tag_inverse a))
+= serialize_synth_eq
+  (* p1 *) (parse_u8
+            `parse_filter`
+            filter_asn1_tag)
+  (* f2 *) (synth_asn1_tag)
+  (* s1 *) (serialize_u8
+            `serialize_filter`
+            filter_asn1_tag)
+  (* g1 *) (synth_asn1_tag_inverse)
+  (* prf*) ()
+  (* in *) (a)
