src/asn1/ASN1.Spec.Tag.fsti
@@ -6,57 +6,52 @@ include LowParse.Spec.Int
 
 include ASN1.Base
 
-/// ASN.1 DER Tag Encoder
-val asn1_tag_of_type: asn1_type -> Tot byte
+val filter_asn1_tag
+  (b: byte)
+: Ghost bool
+  (requires True)
+  (ensures fun r -> r == (b = 0x01uy || b = 0x04uy || b = 0x05uy))
 
-val encode_asn1_tag: asn1_type -> Tot byte
+let valid_asn1_tag_byte = parse_filter_refine filter_asn1_tag
 
-/// Exposing ASN.1 DER Tag kind
-let parse_asn1_tag_kind: parser_kind = constant_size_parser_kind 1
+val synth_asn1_tag
+  (b: parse_filter_refine filter_asn1_tag)
+: Ghost asn1_type
+  (requires True)
+  (ensures fun a ->
+    a == (match b with
+          | 0x01uy -> BOOLEAN
+          | 0x04uy -> OCTET_STRING
+          | 0x05uy -> NULL))
 
+val synth_asn1_tag_inverse
+  (a: asn1_type)
+: Ghost (b: parse_filter_refine filter_asn1_tag{a == synth_asn1_tag b})
+  (requires True)
+  (ensures fun b -> a == synth_asn1_tag b)
 
-/// Generic ASN.1 DER Tag Decoder and Parser/Serializer
-///
-val decode_asn1_tag: s: bytes{Seq.length s == 1} -> Tot (option asn1_type)
+let parse_asn1_tag_kind = strong_parser_kind 1 1 None
+val parse_asn1_tag
+: parser parse_asn1_tag_kind asn1_type
 
-val decode_asn1_tag_injective: unit -> Lemma (
-  forall (s1: bytes {Seq.length s1 == 1})
-    (s2: bytes {Seq.length s2 == 1}).
-  {:pattern (decode_asn1_tag s1); (decode_asn1_tag s2)}
-  let v1, v2 = decode_asn1_tag s1, decode_asn1_tag s2 in
-  (Some? v1 \/ Some? v2) /\ v1 == v2
-    ==> Seq.equal s1 s2)
-
-val parse_asn1_tag: parser parse_asn1_tag_kind asn1_type
-
-val parse_asn1_tag_unfold: input: bytes -> Lemma (
+val parse_asn1_tag_unfold
+  (input: bytes)
+: Lemma (
+  parser_kind_prop parse_asn1_tag_kind parse_asn1_tag /\
   parse parse_asn1_tag input ==
  (match parse parse_u8 input with
-  | Some (x, 1) -> let d = decode_asn1_tag (Seq.create 1 x) in
-                   if Some? d then Some (Some?.v d, 1) else None
-  | _           -> None))
+  | Some (x, consumed) -> if filter_asn1_tag x then
+                          ( Some (synth_asn1_tag x, consumed) )
+                          else
+                          ( None )
+  | None -> None))
 
-val serialize_asn1_tag: unit -> Tot (serializer parse_asn1_tag)
+val serialize_asn1_tag
+: serializer parse_asn1_tag
 
-
-/// Specialized ASN.1 DER Tag Decoder and Parser/Serializer
-///
-val decode_the_asn1_tag: a: asn1_type -> b: bytes{Seq.length b == 1} -> Tot (option (the_asn1_type a))
-
-val decode_the_asn1_tag_injective: a: asn1_type -> Lemma (
-  forall (s1: bytes {Seq.length s1 == 1})
-    (s2: bytes {Seq.length s2 == 1}).
-  {:pattern (decode_the_asn1_tag a s1); (decode_the_asn1_tag a s2)}
-  let v1, v2 = decode_the_asn1_tag a s1, decode_the_asn1_tag a s2 in
-  (Some? v1 \/ Some? v2) /\ v1 == v2
-    ==> Seq.equal s1 s2)
-
-val parse_the_asn1_tag: a: asn1_type -> parser parse_asn1_tag_kind (the_asn1_type a)
-
-val parse_the_asn1_tag_unfold: a: asn1_type -> input: bytes -> Lemma (
-  parse (parse_the_asn1_tag a) input ==
- (match parse parse_u8 input with
-  | Some (x, 1) -> if x = asn1_tag_of_type a then Some (a, 1) else None
-  | _           -> None))
-
-val serialize_the_asn1_tag: a: asn1_type -> Tot (serializer (parse_the_asn1_tag a))
+val serialize_asn1_tag_unfold
+  (a: asn1_type)
+: Lemma (
+  serialize serialize_asn1_tag a
+  `Seq.equal`
+  serialize serialize_u8 (synth_asn1_tag_inverse a))
