src/asn1/ASN1.Low.Base.fst
@@ -1,0 +1,114 @@
+module ASN1.Low.Base
+
+open ASN1.Base
+
+include LowParse.Low.Base
+include LowParse.Low.Combinators
+// include LowParse.Bytes
+
+module U8 = FStar.UInt8
+module U32 = FStar.UInt32
+module HS = FStar.HyperStack
+module HST = FStar.HyperStack.ST
+module MB = LowStar.Monotonic.Buffer
+module B = LowStar.Buffer
+module Cast = FStar.Int.Cast
+open FStar.Integers
+
+let size_t = U32.t
+let byte_t = U8.t
+
+#push-options "--z3rlimit 32"
+/// NOTE: Adapted from `LowParse.Low.Bytes.store_bytes
+inline_for_extraction
+let store_seqbytes
+  (src: bytes)
+  (src_from src_to: size_t)
+  (#rrel #rel: _)
+  (dst: B.mbuffer byte_t rrel rel)
+  (dst_pos: size_t)
+: HST.Stack unit
+  (requires (fun h ->
+    B.live h dst /\
+    v src_from <= v src_to /\ v src_to <= Seq.length src /\
+    v dst_pos + (v src_to - v src_from) <= B.length dst /\
+    writable dst (v dst_pos) (v dst_pos + (v src_to - v src_from)) h
+  ))
+  (ensures (fun h _ h' ->
+    B.modifies (B.loc_buffer_from_to dst dst_pos (dst_pos + (src_to - src_from))) h h' /\
+    writable dst (v dst_pos) (v dst_pos + (v src_to - v src_from)) h' /\
+    Seq.slice (B.as_seq h' dst) (v dst_pos) (v dst_pos + (v src_to - v src_from))
+    `Seq.equal`
+    Seq.slice (src) (v src_from) (v src_to)
+  ))
+= let h0 = HST.get () in
+  HST.push_frame ();
+  let h1 = HST.get () in
+  let bi = B.alloca 0ul 1ul in
+  let h2 = HST.get () in
+  let len = src_to - src_from in
+  C.Loops.do_while
+    (fun h stop ->
+      B.modifies (B.loc_union (B.loc_region_only true (HS.get_tip h1))
+                              (B.loc_buffer_from_to dst dst_pos (dst_pos + len)))
+                              h2 h /\
+      B.live h bi /\
+      writable dst (v dst_pos) (v dst_pos + (v src_to - v src_from)) h /\(
+      let i = Seq.index (B.as_seq h bi) 0 in
+      v i <= v len /\
+      writable dst (v dst_pos) (v dst_pos + v len) h /\
+      Seq.slice (B.as_seq h dst) (v dst_pos) (v dst_pos + v i)
+      `Seq.equal`
+      Seq.slice (src) (v src_from) (v src_from + v i) /\
+      (stop == true ==> i == len)
+    ))
+    (fun _ ->
+      let i = B.index bi 0ul in
+      if i = len then
+      ( true )
+      else
+      ( let x = Seq.index src (v src_from + v i) in
+        mbuffer_upd dst (v dst_pos) (v dst_pos + v len) (dst_pos + i) x
+      ; let i' = i + 1ul in
+        B.upd bi 0ul i'
+      ; (* Prf *) let h' = HST.get () in
+        (* Prf *) Seq.lemma_split (Seq.slice (B.as_seq h' dst) (v dst_pos) (v dst_pos + v i')) (v i)
+      ; i' = len )
+    )
+    ;
+  HST.pop_frame ()
+
+[@unifier_hint_injective]
+inline_for_extraction
+let serializer32_backwards
+  (#k: parser_kind)
+  (#t: Type)
+  (#p: parser k t)
+  (s: serializer p)
+: Tot Type
+= (x: t) ->
+  (#rrel: _) -> (#rel: _) ->
+  (b: B.mbuffer byte_t rrel rel) ->
+  (pos: size_t) ->
+  HST.Stack (offset: size_t)
+  (* NOTE: b[pos] is already written, and b[pos - offset, pos - 1] will be written. *)
+  (requires fun h ->
+    let offset = Seq.length (serialize s x) in
+    B.live h b /\
+    offset <= v pos /\ v pos <= B.length b /\
+    writable b (v pos - offset) (v pos) h)
+  (ensures fun h offset h' ->
+    let sx = serialize s x in
+    let s  = B.as_seq h  b in
+    let s' = B.as_seq h' b in
+    Seq.length sx == v offset /\
+    B.modifies (B.loc_buffer_from_to b (pos - offset) (pos)) h h' /\
+    Seq.slice s 0 (v (pos - offset)) == Seq.slice s' 0 (v (pos - offset)) /\
+    Seq.slice s (v pos) (B.length b) == Seq.slice s' (v pos) (B.length b) /\
+    // (forall (i:nat{0 <= i /\ i < B.length b /\ (i < v (pos - offset) \/ v pos <= i)}).
+    //   let s0 = B.as_seq h b in
+    //   let s1 = B.as_seq h' b in
+    //   s0.[i] == s1.[i]) /\
+    writable b (v (pos - offset)) (v pos) h' /\
+    B.live h' b /\
+    Seq.slice (B.as_seq h' b) (v pos - v offset) (v pos) `Seq.equal` sx)
